deps/poulet4/lib/P4light/Semantics/Typing/Rules.v
@@ -712,22 +712,13 @@ Section Soundness.
         => exists t; cbn; eauto
       end.
 
-    Lemma cast_get_real_type: forall t newt rt,
-        cast_type t newt -> get_real_type ge t = Some rt ->
-        exists realnewt, get_real_type ge newt = Some realnewt.
-    Proof.
-      intros t newt rt Hcast Hreal. revert ge rt Hreal. induction Hcast; intros.
-      - cbn; solve_ex'.
-      - cbn; solve_ex'.
-      - cbn; solve_ex'.
-      - admit.
-      - apply IHHcast in Hreal. destruct Hreal as [realnewt Hrealnewt].
-        cbn. admit.
-        (* destruct t1; try (exfalso; now apply H); *)
-        (*   destruct t2; try (exfalso; now apply H); try (cbn; solve_ex'; easy). *)
-
-    Admitted.
-
+    (* TODO: need
+       - Preservation lemma for eval_cast:
+         [cast_type t1 t2 -> eval_cast t2 v1 = Some v2 -> ⊢ᵥ v1 ∈ t1 -> ⊢ᵥ v2 ∈ t2]
+       - [cast_type x y -> cast_type (normᵗ x) (normᵗ y)]
+       - [eval_cast (normᵗ x) v = eval_cast x v]
+       - [get_real_type ge t1 = Some r1 -> get_real_type ge t2 = Some r2 -> cast_type t1 t2 -> cast_type r1 r2]
+     *)
     Theorem cast_sound : forall tag e t dir,
         cast_type (typ_of_expr e) t ->
         (ge,this,Δ,Γ) ⊢ₑ e ->
@@ -739,14 +730,29 @@ Section Soundness.
       rename H4 into Hokcast; rename H3 into Htoeok; rename H1 into Hokt. clear H2.
       inversion Hise; subst. inversion H4; subst.
       rename H1 into Hist; rename H4 into Hiscast; rename H3 into Hise'. clear H2.
-      pose proof He Hgrt Hdlta as [[v Hev] [Hv Helv]]; eauto.
+      pose proof He Hgrt Hdlta as [[sv Hesv] [Hsv Helsv]]; eauto.
       split; [| split].
-      - clear Helv. destruct (Hv _ Hev) as [rt [Hreal Hvrt]].
-        destruct (exec_val_exists _ Hrob v) as [oldv Hexec].
-        destruct (cast_get_real_type _ _ _ Hcast Hreal) as [realt Hrealt].
-        eexists. eapply exec_expr_cast; eauto.
-        admit.
-      - admit.
+      - clear Helsv. destruct (Hsv _ Hesv) as [rt [Hreal Hsvrt]].
+        destruct (exec_val_exists _ Hrob sv) as [v Hexec].
+        pose proof ok_get_real_type_ex _ _ Hokt _ Hdlta as [r hr].
+        assert (heval_cast: exists newv, eval_cast r v = Some newv).
+        { pose proof exec_val_preserves_typ
+               _ _ _ Hexec _ Hsvrt as Hvrt.
+          assert (hcast : cast_type rt r) by admit.
+          assert (hcast_norm : cast_type (normᵗ rt) (normᵗ r)) by admit.
+          assert (heval_cast_norm: eval_cast (normᵗ r) v = eval_cast r v) by admit.
+          rewrite <- heval_cast_norm.
+          eapply eval_cast_ex; eauto. }
+        firstorder eauto.
+      - clear dependent sv. clear Helsv.
+        intros sv hesv. inv hesv.
+        apply Hsv in H6 as (r & hgetr & holdvr).
+        assert (hnewvr: ⊢ᵥ newv \: normᵗ real_typ) by admit.
+        assert (hsvr: ⊢ᵥ sv \: normᵗ real_typ) by eauto.
+        assert (hcast : cast_type r real_typ) by admit.
+        assert (hcast_norm : cast_type (normᵗ r) (normᵗ real_typ)) by admit.
+        assert (heval_cast_norm: eval_cast (normᵗ real_typ) oldv = eval_cast real_typ oldv) by admit.
+        eauto.
       - intros Hlv; inv Hlv; contradiction.
     Admitted.
 
